{
 "cells": [
  {
   "cell_type": "markdown",
   "metadata": {},
   "source": [
    "# CSCI 5454 Assignment 3 \n",
    "\n",
    "Your Name Here: __ Dania Elmadhun __ "
   ]
  },
  {
   "cell_type": "markdown",
   "metadata": {},
   "source": [
    "## Problem 1: Axioms of Probability (20 points)\n",
    "\n",
    "Let $A$ be a sample space with a set of events $\\{ \\emptyset, E_1, \\ldots, E_n, A \\}$.  We covered the basic axioms\n",
    "of probability in class and recall a few of these axioms here.\n",
    "- $p(\\emptyset) = 0, p(A) = 1$.\n",
    "- $p(E_i) \\geq 0$ and $p(E_i) \\leq 1$ for all events $E_i$.\n",
    "- If $E_1, E_2, \\ldots, E_n$ are pairwise disjoint then $p(E_1 \\cup E_2 \\cup \\cdots \\cup E_n) = p(E_1) + \\cdots + p(E_n) $.\n",
    "\n",
    "Your proof can only use facts about sets, the  axioms above and previously proven facts in this problem. \n",
    "Please write down your proof as a bulleted list as shown below.\n",
    "\n",
    "> __Example__ Prove that if $E_1 \\subseteq E_2$ then $p(E_2 \\setminus E_1) = p(E_2) - p(E_1)$.\n",
    "\n",
    "> __Proof:__  \n",
    "> 1. $E_2 = E_1 \\cup  (E_2 \\setminus E_1) $.\n",
    "> 2. The sets $E_1, (E_2 \\setminus E_1) $ are disjoint. \n",
    "> 3. Therefore, $p(E_2) = p(E_1) + p(E_2 \\setminus E_1)$ (axiom).  \n",
    "> 4. Rearranging, $p(E_2 \\setminus E_1) = p(E_2) - p(E_1)$.\n",
    "\n",
    "(A) Prove that if $E_1 \\subseteq E_2$ then \n",
    "\n",
    "$$p(E_1) \\leq p(E_2)$$.\n",
    "\n",
    "(B) Prove the inclusion-exclusion principle: \n",
    "\n",
    "$$p(E_1 \\cup E_2) = p(E_1) + p(E_2) - p(E_1 \\cap E_2)\\,.$$\n",
    "\n",
    "\n",
    "(C) Prove Boole's Inequality:\n",
    "\n",
    "$$p(E_1) + p(E_2) - 1 \\leq p(E_1 \\cup E_2) \\leq p(E_1) + p(E_2)\\,.$$\n",
    "\n",
    "(D) Prove Frechet's Inequality:\n",
    "\n",
    "$$p(E_1) + p(E_2) -1 \\leq p(E_1 \\cap E_2) \\leq \\min( p(E_1), p(E_2) )\\,. $$\n",
    "\n",
    "\n"
   ]
  },
  {
   "cell_type": "markdown",
   "metadata": {},
   "source": [
    "## Solution (Expected Length: 25 lines)\n",
    "\n",
    "# A\n",
    "\n",
    "Prove that if $E_1 \\subseteq E_2$ then \n",
    "\n",
    "$p(E_1) \\leq p(E_2)$.\n",
    "\n",
    "\n",
    "so $E_1$ is a subset of $E_2$:\n",
    "\n",
    "Proof:\n",
    "\n",
    "1. $E_2=E_1 \\cup (\\bar E_1 \\cap E_2)$\n",
    "\n",
    "meaning: $E_2$ equals the union of $\\bar E_1$ and the intersection of $E_1$ and $E_2$, \n",
    "where $E_1$ and $\\bar E_1 \\cap E_2$ are mutually exclusive\n",
    "\n",
    "2. $P(E_2)=P(E_1)+P(\\bar E_1 \\cap E_2)$\n",
    "\n",
    "\n",
    "if $P(E_1 \\cap E_2)=0$ then $P(E_1 \\cup E_2)=P(E_1)+ P(E_2)$\n",
    "otherwise\n",
    "$P(E_1 \\cap E_2) \\geq 0$\n",
    "\n",
    "\n",
    "3. $P(\\bar E_1 \\cap E_2) \\geq 0$ (axiom)\n",
    "\n",
    "\n",
    "\n",
    "\n",
    "4. Therefore, $p(E_1) \\leq p(E_2)$\n",
    "\n",
    "\n",
    "# B\n",
    "\n",
    "\n",
    "Prove the inclusion-exclusion principle: \n",
    "\n",
    "$p(E_1 \\cup E_2) = p(E_1) + p(E_2) - p(E_1 \\cap E_2)\\,.$\n",
    "\n",
    "Proof:\n",
    "\n",
    "1. $E_1 \\cup E_2=E_1 \\cup E_2\\setminus(E_1 \\cap E_2)$\n",
    "\n",
    "$E_1$ union $E_2$ is a union of two disjoint sets\n",
    "\n",
    "2. $P(E_1 \\cup E_2)=P(E_1\\setminus(E_1\\cap E_2)+P(E_2\\setminus(E_1\\cap E_2)+P(E_1\\cap E_2)$\n",
    "\n",
    "\n",
    "$P(E_2)$ as the union of two disjoint sets\n",
    "\n",
    "3. $P(E_1 \\cup E_2)=P(E_1)-P(E_1\\cap E_2)+P(E_2)-P(E_1\\cap E_2)+P(E_1\\cap E_2)$\n",
    "\n",
    "Simplify and rearrange:\n",
    "\n",
    "4. therefore, we get to the end result:\n",
    "$p(E_1 \\cup E_2) = p(E_1) + p(E_2) - p(E_1 \\cap E_2)\\,.$\n",
    "\n",
    "\n",
    "# C\n",
    "\n",
    "Prove Boole's Inequality:\n",
    "\n",
    "$p(E_1) + p(E_2) - 1 \\leq p(E_1 \\cup E_2) \\leq p(E_1) + p(E_2)\\,.$\n",
    "\n",
    "Proof:\n",
    "\n",
    "From the inclusion-exclusion principle:\n",
    "1. $P(E_1 \\cup E_2) = P(E_1) + P(E_2) - P(E_1 \\cap E_2)\\,.$\n",
    "\n",
    "From the last term of the right side:\n",
    "\n",
    "2. $P(\\bar E_1 \\cap E_2) \\geq 0$ (axiom)\n",
    "\n",
    "if $P(\\bar E_1 \\cap E_2)$ is greater than 0 and the maximum value is 1, we compare to the left side of the equation\n",
    "\n",
    "3. $P(E_1 \\cup E_2) \\geq P(E_1) + P(E_2) - 1 $\n",
    "\n",
    "and this brings us to our final, based on the fact that if $P(\\bar E_1 \\cup E_2)=P(E_1) + P(E_2) - P(E_1 \\cap E_2)\\,$, then $P(\\bar E_1 \\cup E_2) \\geq P(E_1) + P(E_2)$\n",
    "\n",
    "rearrange:\n",
    "\n",
    "4. $p(E_1) + p(E_2) - 1 \\leq p(E_1 \\cup E_2) \\geq p(E_1) + p(E_2)\\,.$\n",
    "\n",
    "\n",
    "# D\n",
    "\n",
    "Prove Frechet's Inequality:\n",
    "\n",
    "$p(E_1) + p(E_2) -1 \\leq p(E_1 \\cap E_2) \\leq \\min( p(E_1), p(E_2) )\\, $\n",
    "\n",
    "Proof:\n",
    "\n",
    "Same concept of part (c)\n",
    "\n",
    "taking the inclusion-exclusion principle:\n",
    "1. $P(E_1 \\cup E_2) = P(E_1) + P(E_2) - P(E_1 \\cap E_2)\\,.$\n",
    "\n",
    "\n",
    "if we switch around the equation:\n",
    "\n",
    "$P(E_1 \\cap E_2) = P(E_1) + P(E_2) - P(E_1 \\cup E_2)\\,.$\n",
    "\n",
    "\n",
    "because the union of $P(E_1)$ and $P(E_2)$ is equal to 1, \n",
    "\n",
    "$P( E_1 \\cup E_2) = 1$\n",
    "then (using the same concept as we used in the Boole's Inequality),\n",
    "\n",
    "2. $p(E_1) + p(E_2) -1 \\leq p(E_1 \\cap E_2)$\n",
    "\n",
    "in the intersection of $P(E_1)$ and $P(E_2)$, the intersection cannot be more than the smallest value of $P(E_1)$ and $P(E_2)$, meaning:\n",
    "\n",
    "$P(E_1 \\cap E_2) \\leq P(E_1)$\n",
    "\n",
    "and\n",
    "\n",
    "$P(E_1 \\cap E_2) \\leq P(E_2)$\n",
    "\n",
    "which is the same as the upper bound:\n",
    "\n",
    "3. $P(E_1 \\cap E_2) \\leq \\min( p(E_1), p(E_2) )$\n",
    "\n",
    "Putting them together:\n",
    "\n",
    "4. $p(E_1) + p(E_2) -1 \\leq p(E_1 \\cap E_2) \\leq \\min( p(E_1), p(E_2) )$\n",
    "\n",
    "\n",
    "\n"
   ]
  },
  {
   "cell_type": "markdown",
   "metadata": {},
   "source": [
    "## Problem 2 (10 points)\n",
    "\n",
    "Let $X$ be a random variable that takes values in the range $\\{ 0, \\ldots, n \\} $. Show that \n",
    "\n",
    "$$ \\mathbb{E}(X) = \\sum_{i=1}^n \\mathbb{P}( X \\geq i ) = \\mathbb{P}( X \\geq 1 ) +  \\mathbb{P}( X \\geq 2  ) + \\cdots + \\mathbb{P}(X \\geq n) $$.\n",
    "\n",
    "__Hint:__ Note that $\\mathbb{E}(X) = 1 \\mathbb{P}(X = 1) + 2 \\mathbb{P}( X = 2) + \\cdots + n \\mathbb{P}(X = n)$. Show that the RHS of the equality is exactly this."
   ]
  },
  {
   "cell_type": "markdown",
   "metadata": {},
   "source": [
    "## Answer (Expected length: 6 lines)\n",
    "\n",
    "Prove:\n",
    "$ \\mathbb{E}(X) = \\sum_{i=1}^n \\mathbb{P}( X \\geq i ) = \\mathbb{P}( X \\geq 1 ) +  \\mathbb{P}( X \\geq 2  ) + \\cdots + \\mathbb{P}(X \\geq n) $\n",
    "\n",
    "$ \\mathbb{E}(X) = \\sum_{i=1}^n \\mathbb{P}( X \\geq i )$\n",
    "\n",
    "HINT:\n",
    "\n",
    "$\\mathbb{E}(X) = 1 \\mathbb{P}(X = 1) + 2 \\mathbb{P}( X = 2) + \\cdots + n \\mathbb{P}(X = n)$\n",
    "\n",
    "show that the right hand side of the equality is the same as above:\n",
    "\n",
    "$1 \\mathbb{P}(X = 1) + 2 \\mathbb{P}( X = 2) + \\cdots + n \\mathbb{P}(X = n)=\\mathbb{P}( X \\geq 1 ) +  \\mathbb{P}( X \\geq 2  ) + \\cdots + \\mathbb{P}(X \\geq n) $\n",
    "\n",
    "\n",
    "if we look at $\\mathbb{P}(X \\geq 1)$:\n",
    "\n",
    "we sum all of the values equal to 1 or above:\n",
    "\n",
    "$P(X \\geq 1)=P(x=1)+P(x=2)+P(x=3)+...+P(x=n)$\n",
    "\n",
    "we do the same for $\\mathbb{P}(X \\geq 2)$ and so on:\n",
    "\n",
    "$P(X \\geq 2)=P(x=2)+P(x=3)+...+P(x=n)$\n",
    "\n",
    "$P(X \\geq 3)=P(x=3)+P(x=4)+...+P(x=n)$\n",
    "\n",
    "if we sum all of these equations for each equality we get the final answer:\n",
    "\n",
    "\n",
    "$\\mathbb{E}(X)= \\sum_{i=1}^n P(X \\geq i)=1 \\times P(x=1)+2 \\times P(x=2) +...+n \\times P(x=n)$\n",
    "\n"
   ]
  },
  {
   "cell_type": "markdown",
   "metadata": {},
   "source": [
    "## Problem 3 (15 points)\n",
    "\n",
    "We draw two numbers independently and uniformly at random  from the set $\\{1, \\ldots, n\\}$ with replacement (i.e, the same number can be drawn twice). What is the expected value of the minimum of these two numbers? Show that this number is  $\\frac{n}{3} + O(1) $.\n",
    "\n",
    "\n",
    "\n",
    "__Hint:__ First calculate the probability that the smaller of the two numbers is $\\geq j$ for each $j \\in \\{ 1, \\ldots, n\\}$. Next use the result from the previous problem. Also note that $1^2 + 2^2 + \\cdots + n^2 = \\frac{n(n+1)(2n+1)}{6}$.\n",
    "\n",
    "__(B)__ Repeat the same calculation for the maximum of the two numbers.\n",
    "\n"
   ]
  },
  {
   "cell_type": "markdown",
   "metadata": {},
   "source": [
    "### Answer (Expected Length: 6 lines).\n",
    "\n",
    "# A\n",
    "\n",
    "Show that the expected value of the minimum of the two randomly drawn numbers is $\\frac{n}{3} + O(1) $\n",
    "\n",
    "From Problem 2:\n",
    "\n",
    "$E(X)= \\sum_{i=1}^n P(X \\geq i)$\n",
    "\n",
    "the minimum of two choices worked into the equation:\n",
    "\n",
    "$\\sum_{i=1}^n P(X \\geq i) -> P(min(x_1,x_2) \\geq j)$\n",
    "\n",
    "Therefore\n",
    "\n",
    "$E(min(x_1,x_2))=\\sum_{j=1}^n P(min(x_1,x_2) \\geq j)$\n",
    "\n",
    "which is the same as:\n",
    "\n",
    "$P(min(x_1,x_2) \\geq j)=P(x_1 \\geq j) \\times P(x_2 \\geq j)$\n",
    "\n",
    "to turn this into an equation:\n",
    "\n",
    "the probability of $x_1$ or $x_2$ is greater than j of a given set n\n",
    "\n",
    "$=\\sum_{j=1}^n \\left( \\frac{n-(j-1)}{n}\\right)^2$\n",
    "\n",
    "we take out the constant in the equation:\n",
    "\n",
    "$=\\frac{1}{n^2}\\sum_{j=1}^n (n-j+1)^2$\n",
    "\n",
    "expanded (and reversed):\n",
    "\n",
    "$=\\frac{1}{n^2}[n^2+(n-1)^2+...+2^2+1^2 ]$\n",
    "\n",
    "simplified from the hint:\n",
    "\n",
    "$=\\frac{n(n+1)(2n+1)}{6n^2}$\n",
    "\n",
    "$=\\frac{2n^2+3n+1}{6n}$\n",
    "\n",
    "$=\\frac{n}{3}+\\frac{1}{2}+\\frac{1}{6n}$\n",
    "\n",
    "for the 3rd term, as n approaches infinity $\\frac{1}{6n}$ and the constant $\\frac{1}{2}$ can be simplified to $O(1)$\n",
    "\n",
    "so the term goes to:\n",
    "\n",
    "$\\frac{n}{3} + O(1) $\n",
    "\n",
    "\n",
    "# B\n",
    "\n",
    "changing to the maximum of the two numbers:\n",
    "\n",
    "$E(max(x_1,x_2))=\\sum_{j=1}^n P(max(x_1,x_2) \\geq j)$\n",
    "\n",
    "another way to write the max in the same way we did as part A\n",
    "\n",
    "$\\sum_{j=1}^n P(max(x_1,x_2) \\geq j)=1-P(x_1 <j) \\times P(x_2 <j)$\n",
    "\n",
    "the probability of $x_1$ or $x_2$ is greater than j of a given set n\n",
    "\n",
    "$=\\sum_{j=1}^n 1-\\left( \\frac{j-1}{n}\\right)^2$\n",
    "\n",
    "take out the constant\n",
    "\n",
    "$=n-\\frac{1}{n^2}\\sum_{j=1}^n (j-1)^2$\n",
    "\n",
    "simplified:\n",
    "\n",
    "$=n-\\frac{1}{n^2}(0^2+1^2+2^2+...+(n-1)^2)$\n",
    "\n",
    "$=n-\\frac{1}{n^2} \\left( \\frac{(n-1)(n)(2n-1)}{6} \\right)$\n",
    "\n",
    "$=n-\\left( \\frac{(n-1)(2n-1)}{6n} \\right)$\n",
    "\n",
    "$=\\frac{6n^2}{6n}-\\left( \\frac{(n-1)(2n-1)}{6n} \\right)$\n",
    "\n",
    "$=\\left( \\frac{6n^2-2n^2+3n-1}{6n} \\right)$\n",
    "\n",
    "$=\\frac{4n^2}{6n}+\\frac{3n}{6n}-\\frac{1}{6n}$\n",
    "\n",
    "$=\\frac{2n}{3}+\\frac{1}{2}-\\frac{1}{6n}$\n",
    "\n",
    "so the term goes to:\n",
    "\n",
    "$\\frac{2n}{3} + O(1) $"
   ]
  },
  {
   "cell_type": "markdown",
   "metadata": {},
   "source": [
    "## Problem 4  (10 points)\n",
    "\n",
    "\n",
    "Alice and Bob play the following game by tossing a fair (unbiased) coin. Each player takes turns starting with Alice's turn.\n",
    "- If Alice turns up heads she wins at once, or else Bob gets a turn.\n",
    "- If Bob turns up tails, he wins at once, or else Alice gets a turn.\n",
    "\n",
    "What is the probability that Alice wins?  What is the expected number of  tosses in the game?\n",
    "\n",
    "__(B, extra credit)__ Design a game between Alice and Bob where the probability that Bob wins is precisely $\\frac{21}{64}$. In each move of the game, you must specify which player gets a turn and what happens if that player wins a heads or a tails.\n",
    "\n"
   ]
  },
  {
   "cell_type": "markdown",
   "metadata": {},
   "source": [
    "### Answer (Expected Length: 4 lines).\n",
    "\n",
    "# A\n",
    "\n",
    "# What is the probability Alice wins?\n",
    "\n",
    "based on the rules, the following probabilities are the possible wins alice can get:\n",
    "\n",
    "$P(A)=P(h)+(t,h,h)+P(t,h,t,h,h)+...$\n",
    "\n",
    "we translate this into:\n",
    "\n",
    "$P(A)=\\frac{1}{2}+\\frac{1}{2^3}+\\frac{1}{2^5}+....$\n",
    "\n",
    "take out $\\frac{1}{2}$\n",
    "\n",
    "$P(A)=\\frac{1}{2}\\left(1+\\frac{1}{2^2}+\\frac{1}{2^4}+....\\right)$\n",
    "\n",
    "infinite geometric series common ratio, r for r < 1:\n",
    "\n",
    "$convergence=\\frac{1}{1-r}$\n",
    "\n",
    "$r=\\frac{1}{2^2}$\n",
    "\n",
    "simplified to:\n",
    "\n",
    "$P(A)=\\frac{1}{2} \\times \\frac {1}{1-\\frac{1}{2^2}}$\n",
    "\n",
    "Simplified:\n",
    "\n",
    "\n",
    "$P(A)=\\frac{1}{2} \\times \\frac {4}{3}$\n",
    "\n",
    "# Final Answer:\n",
    "\n",
    "$P(A)=\\frac{2}{3}$\n",
    "\n",
    "\n",
    "# What is the expected number of tosses in the game?\n",
    "\n",
    "first we define the probabilities of the different outcomes that will end the game\n",
    "\n",
    "$E(x)=1P(h)+2P(h,t)+3P(h,h,h)+...$\n",
    "\n",
    "insert real probability values:\n",
    "\n",
    "\n",
    "$E(x)=1 \\times \\frac{1}{2}+2 \\times \\frac{1}{2^2}+3 \\times \\frac{1}{2^3}+...$\n",
    "\n",
    "$E(x)=\\sum_{i=1}^{\\inf} \\frac {i}{2^i}$\n",
    "\n",
    "pull out $\\frac{1}{2}$\n",
    "\n",
    "\n",
    "$\\frac{E(x)}{2}=1 \\times \\frac{1}{2^2}+2 \\times \\frac{2}{2^3}+3 \\times \\frac{1}{2^4}+...$\n",
    "\n",
    "infinite geometric series simplifies to:\n",
    "\n",
    "$\\frac{E(x)}{2}=\\frac{1}{2} \\times \\left(\\frac {1}{1-\\frac{1}{2}}\\right)$\n",
    "\n",
    "expected tosses are:\n",
    "\n",
    "$E(x)=2$\n",
    "\n",
    "\n",
    "# Extra Credit\n",
    "\n",
    "__Shout out to Ilam for helping get to this solution__\n",
    "\n",
    "\n",
    "Game between alice and bob where $P(B)=\\frac{21}{64}$\n",
    "\n",
    "disect the probability and break it down into parts that would match the possible wins(denominator):\n",
    "\n",
    "$P(B)=\\frac{21}{64}=\\frac{21}{2^6}$\n",
    "\n",
    "break up the numerator into power of 2(under the value 21 obviously) with a pattern similar to the probabilities in the question(odd, evens):\n",
    "\n",
    "$2^0=1, 2^1=2, 2^2=4, 2^3=8, 2^4=16$\n",
    "\n",
    "Hold this thought. \n",
    "\n",
    "if we limit the number of possible games and keep the rules all the same:\n",
    "\n",
    "Each player takes turns starting with Alice's turn.\n",
    "\n",
    "-If Alice turns up heads she wins at once, or else Bob gets a turn.\n",
    "\n",
    "-If Bob turns up tails, he wins at once, or else Alice gets a turn.\n",
    "\n",
    "There can only be a total of 6 coin tosses between Alice and Bob.\n",
    "If max coin tosses is reached, no one wins. \n",
    "\n",
    "therefore the probability of Bob winning is defined as:\n",
    "\n",
    "$P(B)=P(t,t)+P(t,h,t,t)+P(t,h,t,h,t,t)$\n",
    "\n",
    "$P(B)=\\frac{1}{2^2}+\\frac{1}{2^4}+\\frac{1}{2^6}$ \n",
    "\n",
    "$P(B)=\\frac{1}{4}+\\frac{1}{16}+\\frac{1}{64}$ \n",
    "\n",
    "$P(B)=\\frac{21}{64}$\n",
    "\n",
    "\n",
    "for kicks:\n",
    "\n",
    "$P(A)=P(h)+P(t,h,h)+P(t,h,t,h,h)$\n",
    "\n",
    "$P(A)=\\frac{1}{2^1}+\\frac{1}{2^3}+\\frac{1}{2^5}$ \n",
    "\n",
    "$P(A)=\\frac{1}{2}+\\frac{1}{8}+\\frac{1}{32}$\n",
    "\n",
    "$P(A)=\\frac{1}{2}+\\frac{1}{8}+\\frac{1}{32}$\n",
    "\n",
    "$P(A)=\\frac{21}{32}=\\frac{42}{64}$\n",
    "\n",
    "NW=no win\n",
    "\n",
    "$P(NW)=P(t,h,t,h,t)$\n",
    "\n",
    "$P(NW)=\\frac{1}{2^6}$\n",
    "\n",
    "$P(NW)=\\frac{1}{64}$\n",
    "\n",
    "check probs:\n",
    "\n",
    "$P(A)+P(B)+P(NW)=\\frac{21}{64}+\\frac{42}{64}+\\frac{1}{64}=1$\n"
   ]
  },
  {
   "cell_type": "code",
   "execution_count": null,
   "metadata": {},
   "outputs": [],
   "source": []
  }
 ],
 "metadata": {
  "kernelspec": {
   "display_name": "Python 3",
   "language": "python",
   "name": "python3"
  },
  "language_info": {
   "codemirror_mode": {
    "name": "ipython",
    "version": 3
   },
   "file_extension": ".py",
   "mimetype": "text/x-python",
   "name": "python",
   "nbconvert_exporter": "python",
   "pygments_lexer": "ipython3",
   "version": "3.6.5"
  }
 },
 "nbformat": 4,
 "nbformat_minor": 2
}
